@prefix rdf: <http://www.w3.org/1999/02/22-rdf-syntax-ns#> .
@prefix dct:<http://purl.org/dc/terms/> .
@prefix rdfs: <http://www.w3.org/2000/01/rdf-schema#> .
@prefix owl: <http://www.w3.org/2002/07/owl#> .
@prefix odette: <https://vocab.eccenca.com/odette/> .
@prefix xsd:<http://www.w3.org/2001/XMLSchema#> .
@prefix foaf:<http://xmlns.com/foaf/0.1/> .
@prefix vann:<http://purl.org/vocab/vann/>.

odette: a owl:Ontology;
  rdfs:label "ODETTE";
  rdfs:comment "An RDF vocabulary representing the ODETTE Business Entity Administration schema.";
  foaf:maker <http://sebastian.tramp.name>;
  vann:preferredNamespacePrefix "odette";
  vann:preferredNamespaceUri "https://vocab.eccenca.com/odette/";
  foaf:homepage <https://github.com/vocol/odette>;
  foaf:primaryTopic odette:BusinessEntity;
  vann:changes <https://github.com/vocol/odette/commits/master>;
  .

odette:type a owl:DatatypeProperty;
  rdfs:subPropertyOf dct:description;
  rdfs:label "ODETTE Type Information";
  .

odette:occurrence a owl:DatatypeProperty;
  rdfs:subPropertyOf dct:description;
  rdfs:label "ODETTE Occurrence Information";
  .

odette:Country a owl:Class;
  rdfs:subClassOf <http://www.geonames.org/ontology#Country>;
  rdfs:label "Country";
  .

odette:Feature a owl:Class;
  rdfs:subClassOf <http://www.geonames.org/ontology#Feature>;
  rdfs:label "Feature";
  .

odette:Document a owl:Class;
  rdfs:subClassOf foaf:Document;
  rdfs:label "Document";
  .

#D - Business Entity
#D -   Universal Party ID
#D -   Direct Parent ID
#D -   Domestic Ultimate Parent ID
#D -   Global Ultimate Parent ID
#E -   Previous Universal Party ID
#E -   Entity Type
#E -   Functional Entity Type
#D -   Homepage
#D -   Name
#D -   Trade Name
#E -   Previous Name

odette:BusinessEntity a owl:Class;
  rdfs:comment "When adding, changing, or deactivating a Business Entity, only one Business Entity shall be included in an administration message, in case of a response to a 'request information' message the Business Entity is repeatable to allow the transmission of all relevant sub-entities.";
  dct:description """Business Entity denominates any organisational unit within a company, ranging from the legal head office or headquarters down to a sales office or unloading dock. The Business Entity record contains all data for the organisational unit that is relevant to exchanges between business partners.
Business entities may be described as Registered or Non-Registered.
Registered entities are those organisational units which have been allocated a unique registration number by an appropriate registration authority (e.g. Dun & Bradstreet). Non-Registered entities are those organisational units which have not been allocated such a unique registration number.
Each Business Entity (Registered or Non-Registered) will have a Universal Party ID (UPI) which is constructed according to the Odette Recommendation based on ISO6523 rules.
The UPI consists of 3 segments and for Non-Registered entities the first two segments of the UPI will be identical to those of the UPI of their associated Registered entity. Records for Non- Registered entities may therefore only be created when a record for the associated Registered Entity already exists.
Each Business Entity (Registered or Non-Registered) may also be associated with other Business Entities through separate links within the Business Entity record (e.g. direct parent ID, functional reference etc.).
""";
  rdfs:label "Business Entity";
  .

odette:LegalHeadOffice a owl:Class;
  rdfs:subClassOf odette:BusinessEntity;
  rdfs:comment "equals to entity-type 001";
  rdfs:label "Legal Head Office";
  .

odette:OtherRegisteredEntity a owl:Class;
  rdfs:subClassOf odette:BusinessEntity;
  rdfs:comment "equals to entity-type 002";
  rdfs:label "Other Registered Entity";
  .

odette:NonRegisteredEntity a owl:Class;
  rdfs:subClassOf odette:BusinessEntity;
  rdfs:comment "equals to entity-type 003";
  rdfs:label "Non-Registered Entity";
  .

odette:officeLocation a owl:ObjectProperty;
  rdfs:domain odette:LegalHeadOffice;
  rdfs:range odette:BusinessEntity;
  rdfs:label "Office Location";
  .

odette:homepage a owl:DatatypeProperty;
  dct:description "Topmost URL of the entity";
  odette:type "XSD Data types::string";
  odette:occurrence "0..1";
  rdfs:label "Homepage";
  .

odette:name a owl:DatatypeProperty;
  odette:type "Main::core::String..90";
  odette:occurrence "0 .. unbounded";
  dct:description "Name of the entity";
  rdfs:comment """The attribute can be repeated in various languages. A maximum of 1 line per language is recommended.
For B2B processes (in XML messages), this information may be transmitted with a language attribute and is repeatable.
For creation or change of business entity data, this field is required.""";
  rdfs:label "Name";
  .

odette:tradeName a owl:DatatypeProperty;
  odette:type "Main::core::String..90";
  dct:description "Marketing or brand name, may be different to the legal name";
  rdfs:comment """The attribute can be repeated in various languages. A maximum of 1 line per language is recommended.
For B2B processes (in XML messages), this information may be transmitted with a language attribute and is repeatable.""";
  odette:occurrence "0..unbounded";
  rdfs:label "Trade Name";
  .

odette:previousName a owl:DatatypeProperty;
  odette:type "Main::core::String..90";
  dct:description "Previously used name of the entity.";
  rdfs:comment """The attribute can be repeated in various languages. A maximum of 1 line per language is recommended.
For B2B processes (in XML messages), this information may be transmitted with a language attribute and is repeatable.""";
  rdfs:label "Previous Name";
  .


#D -   Address
#D -      Street
#D -      City
#D -      Post Code
#D -      Post Box ID
#D -      Post Code POBox
#D -      Sub Country Code
#D -      Address Line Text
#D -      Country Code
#D -      Time Zone

odette:address a owl:ObjectProperty;
  rdfs:domain odette:BusinessEntity;
  rdfs:range odette:Address;
  rdfs:label "(Main) Address";
  .

odette:mailingAddress a owl:ObjectProperty;
  rdfs:domain odette:BusinessEntity;
  rdfs:range odette:Address;
  rdfs:label "Mailing Address";
  .

odette:Address a owl:Class;
  dct:description """Physical address incl. street or building ID. For a legal head office, this address is the legal address as registered within commercial registers. For B2B processes (in XML messages), language dependent parts of the address may be transmitted with a language attribute and are repeatable.""";
  rdfs:comment """Recommeded usage:
Variant 1: Structured address
Street, Post Code, City, Country Code
Variant 2: Structured Address
Post Box ID, Post Code POBox, City, Country Code
For creation or change of business entity data, this field is required.""";
  rdfs:label "Address";
  .

odette:street a owl:DatatypeProperty;
  odette:type "Main::core::String..35";
  odette:occurrence "0 .. unbounded";
  dct:description "The name that identifies the location of a house or building: usually within a street as part of an address.";
  rdfs:comment "For B2B processes (in XML messages), this information may be transmitted with a language attribute and is repeatable. A maximum of 2 lines per language is recommended.";
  rdfs:label "Street";
  .

odette:city a owl:DatatypeProperty;
  odette:type "Main::core::String..35";
  odette:occurrence "1 .. unbounded";
  dct:description """The name of the city, town, or village of this address.""";
  rdfs:comment """For B2B processes (in XML messages), this information may be transmitted with a language attribute and is repeatable. One line per language is recommended.""";
  rdfs:label "City";
  .

odette:postCode a owl:DatatypeProperty;
  odette:type "Main::core::String..9";
  odette:occurrence "0..1";
  dct:description """The identifier for one or more properties according to the postal service of that country; a group of letters and/or numbers added to the postal address to assist in the sorting of mail.""";
  rdfs:label "Post Code";
  .

odette:postBoxId a owl:DatatypeProperty;
  odette:type "Main::core::String..35";
  odette:occurrence "0..1";
  dct:description """Identifier of a post box according to the national postal services.""";
  rdfs:label "Post Box ID";
  .

odette:postCodePoBox a owl:DatatypeProperty;
  odette:type "Main::core::String..9";
  odette:occurrence "0..1";
  dct:description """The identifier for a post box according to the postal service of that country; a group of letters and/or numbers added to the postal address to assist in the sorting of mail.""";
  rdfs:label "Post Code POBox";
  .

odette:subCountryCode a owl:DatatypeProperty;
  odette:type "Main::core::String..9";
  odette:occurrence "0..1";
  dct:description """State or region within a country. The use of ISO 3166-2 is recommended.""";
  rdfs:seeAlso <http://www.unece.org/cefact/locode/service/main.htm>, <http://www.iso.org/iso/en/prods-services/iso3166ma/index.html>;
  rdfs:label "Sub Country Code";
  .

odette:addressLineText a owl:DatatypeProperty;
  odette:type "Main::core::String..35";
  odette:occurrence "0 .. unbounded";
  dct:description """A text line containing non-structured address information.""";
  rdfs:comment """Repeatable in various languages, a maximum number of 5 lines per language is recommended.""";
  rdfs:label "Address Line Text";
  .

odette:countryCode a owl:DatatypeProperty;
  odette:type "Main::core::Country Code";
  odette:occurrence "1..1";
  dct:description """Provides the country part of an address using a code.
Use ISO3166 two alpha code.""";
  rdfs:seeAlso <http://www.unece.org/cefact/locode/service/main.htm>,<http://www.iso.org/iso/en/prods-services/iso3166ma/index.html>;
  rdfs:label "Country Code";
  .

odette:timeZone a owl:DatatypeProperty;
  odette:type "Main::core::String..10";
  odette:occurrence "0..1";
  dct:description """Time zone as difference to UTC e.g. UTC+01:00""";
  rdfs:label "Time Zone";
  .

#D -   General Contact
#D -      Telephone Number
#D -      Fax Number
#D -      Email Address
#D -      Preferred Language

odette:telephoneNumber a owl:DatatypeProperty;
  odette:type "Main::core::String..100";
  odette:occurrence "1..1";
  dct:description """The number or virtual 'address' of a telephone in a telecommunication system""";
  rdfs:label "Telephone Number";
  .

odette:faxNumber a owl:DatatypeProperty;
  odette:type "Main::core::String..100";
  odette:occurrence "0..1";
  dct:description """The number or virtual 'address' of a facsimile in a telecommunication system""";
  rdfs:label "Fax Number";
  .

odette:emailAddress a owl:DatatypeProperty;
  odette:type "Main::core::String..100";
  odette:occurrence "0..1";
  dct:description """The number or virtual 'address' of an e-mail mailbox in the internet or other network.""";
  rdfs:label "Email Address";
  .


#odette:generalContact a owl:ObjectProperty;
#  rdfs:domain odette:BusinessEntity;
#  rdfs:range odette:Contact;
#  rdfs:label "General Contact".

#D -   Legal Entity Details
#D -      Place Of Jurisdiction
#D -      Legal Form
#D -          Legal Form Code
#D -          Legal Form Text
#E -      Registered Capital
#E -          Amount Value
#E -          Currency Code
#E -      Minority Business Enterprise
#E -          Minority Owned Business Identification Code
#E -          Certifying Agency
#E -          Certificate Expiration Date
#E -   Tax Registration Details
#E -      VAT Registration ID
#E -      Fiscal Registration ID
#E -   Bank Account Details
#E -        Currency Code
#E -        Account Holder Name
#E -        Bank Identification
#E -           Bank Branch ID
#E -           Agency
#E -           Code List ID
#E -           Bank Name
#E -           City
#E -           Country Code
#E -           SWIFT Code

odette:isClientOf a owl:ObjectProperty;
  rdfs:domain odette:LegalHeadOffice;
  rdfs:range odette:LegalHeadOffice;
  rdfs:label "is client of";
  .

odette:isSupplierOf a owl:ObjectProperty;
  rdfs:domain odette:LegalHeadOffice;
  rdfs:range odette:LegalHeadOffice;
  rdfs:label "is supplier of";
  .

odette:lastUpdate a owl:DatatypeProperty;
  rdfs:range xsd:dateTime;
  rdfs:label "last update";
  .

odette:logo a owl:ObjectProperty;
  rdfs:subPropertyOf foaf:logo;
  rdfs:label "logo";
  .

odette:billingAddress a owl:ObjectProperty;
  rdfs:domain odette:LegalHeadOffice;
  rdfs:range odette:Address;
  rdfs:label "Billing Address";
  .

odette:additionalLink a owl:DatatypeProperty;
  rdfs:domain odette:LegalHeadOffice;
  rdfs:range odette:Document;
  rdfs:label "additional link";
  .

odette:standardFormContract a owl:ObjectProperty;
  rdfs:domain odette:LegalHeadOffice;
  rdfs:range odette:Document;
  rdfs:label "Standard form contract";
  .

odette:vATRegistrationId a owl:DatatypeProperty;
  dct:description "Unique number assigned by the relevant tax authority to identify a party for use in relation to Value Added Tax (VAT).";
  rdfs:domain odette:LegalHeadOffice;
  rdfs:label "VAT Registration ID";
  .

odette:fiscalRegistrationId a owl:DatatypeProperty;
  dct:description "Tax payer's number. Number assigned to individual persons as well as to corporates by a public institution; this number is different from the VAT registration number.";
  rdfs:domain odette:LegalHeadOffice;
  rdfs:label "Fiscal Registration ID";
  .


